PsNat.v
@@ -6,71 +6,71 @@ Require Import Omega.
 Require Import Listutils.
 Require Import PsCore.
 
-Definition termincr : term := term_list
-  [ term_dup ; term_quote ; term_swap ; term_quote ; term_cons ;
-    term_swap ; term_quote ; term_cons ; term_exec ;
-    term_snoc ; term_swap ].
+Definition termincr : term := termlist
+  [ termdup ; termquote ; termswap ; termquote ; termcons ;
+    termswap ; termquote ; termcons ; termexec ;
+    termsnoc ; termswap ].
 
 Lemma eval_termincr : forall (t1 t2 : term) (vs ps : stack),
-  (t1 :: t2 :: vs, termincr :: ps) |=>* (t1 :: term_seq t2 t1 :: vs, ps).
+  (t1 :: t2 :: vs, termincr :: ps) |=>* (t1 :: termseq t2 t1 :: vs, ps).
   intros ; evalauto.
 Qed.
 
 Lemma eval_termincr_replicate : forall (n : nat) (t1 t2 : term) (vs ps : stack),
   (t1 :: t2 :: vs, replicate n termincr ++ ps) |=>*
-    (t1 :: term_list' (replicate n t1) t2 :: vs, ps).
+    (t1 :: termlist' (replicate n t1) t2 :: vs, ps).
   induction n ; intros ; evalauto.
   evalpartial IHn ; evalauto.
 Qed.
 
-Definition termnatq (n : nat) : term := term_list (replicate n termincr).
+Definition termnatq (n : nat) : term := termlist (replicate n termincr).
 
 Lemma eval_termnatq : forall (n : nat) (t1 t2 : term) (vs ps : stack),
   (t1 :: t2 :: vs, termnatq n :: ps) |=>*
-    (t1 :: term_list' (replicate n t1) t2 :: vs, ps).
+    (t1 :: termlist' (replicate n t1) t2 :: vs, ps).
   intros.
-  evalpartial eval_term_list.
+  evalpartial eval_termlist.
   evalpartial eval_termincr_replicate.
   evalauto.
 Qed.
 
-Definition termnat (n : nat) (t1 : term) : Prop :=
+Definition termnat_spec (n : nat) (t1 : term) : Prop :=
   forall (t2 : term) (vs ps : stack),
     (t2 :: vs, t1 :: ps) |=>* (vs, replicate n t2 ++ ps).
 
-Definition termnat_term (n : nat) : term := term_list
-  [ term_push ; termnop ; term_swap ; termnatq n ; term_pop ; term_exec ].
+Definition termnat (n : nat) : term := termlist
+  [ termpush ; termnop ; termswap ; termnatq n ; termpop ; termexec ].
 
-Lemma eval_termnat_term : forall (n : nat), termnat n (termnat_term n).
+Lemma eval_termnat : forall (n : nat), termnat_spec n (termnat n).
   repeat intro.
-  evalpartial eval_term_list ; evalauto.
+  evalpartial eval_termlist ; evalauto.
   evalpartial eval_termnatq ; evalauto.
-  apply eval_term_list.
+  apply eval_termlist.
 Qed.
 
-Definition termnat_quote : term := term_list
-  [ term_push ; termnop ; term_quote ;
-    term_push ; termincr ; term_quote ; term_cons ;
-    term_swap ; term_quote ; term_cons ; term_exec ;
-    term_push ; termincr ; term_swap ; term_exec ; term_pop ].
+Definition termnat_quote : term := termlist
+  [ termpush ; termnop ; termquote ;
+    termpush ; termincr ; termquote ; termcons ;
+    termswap ; termquote ; termcons ; termexec ;
+    termpush ; termincr ; termswap ; termexec ; termpop ].
 
 Lemma eval_termnat_quote : forall (n : nat) (t : term) (vs ps : stack),
-  termnat n t -> (t :: vs, termnat_quote :: ps) |=>* (termnatq n :: vs, ps).
+  termnat_spec n t -> (t :: vs, termnat_quote :: ps) |=>* (termnatq n :: vs, ps).
   repeat intro.
   evalauto ; evalpartial H ; evalpartial eval_termincr_replicate ; evalauto.
 Qed.
 
-Definition termnat_unquote : term := term_list
-  [ term_push ; termnop ;
-    term_push ; term_push ; term_cons ;
-    term_push ; termnop ; term_cons ;
-    term_push ; term_swap ; term_cons ;
-    term_snoc ;
-    term_push ; term_pop ; term_cons ;
-    term_push ; term_exec ; term_cons ].
+Definition termnat_unquote : term := termlist
+  [ termpush ; termnop ;
+    termpush ; termpush ; termcons ;
+    termpush ; termnop ; termcons ;
+    termpush ; termswap ; termcons ;
+    termsnoc ;
+    termpush ; termpop ; termcons ;
+    termpush ; termexec ; termcons ].
 
 Definition eval_termnat_unquote : forall (n : nat) (vs ps : stack),
-  (termnatq n :: vs, termnat_unquote :: ps) |=>* (termnat_term n :: vs, ps).
+  (termnatq n :: vs, termnat_unquote :: ps) |=>* (termnat n :: vs, ps).
   repeat intro ; evalauto.
 Qed.
 
@@ -78,57 +78,54 @@ Lemma termnatq_eqmap : forall (n m : nat), termnatq n = termnatq m -> n = m.
   intro.
   induction n ; intros ; destruct m.
   auto.
-  unfold termnatq, term_list, replicate at 1, term_list' at 1, fold_left in H.
-  rewrite (term_list_replicate (S m) termincr termnop) in H.
+  unfold termnatq, termlist, replicate at 1, termlist' at 1, fold_left in H.
+  rewrite (termlist_replicate (S m) termincr termnop) in H.
   inversion H.
-  unfold termnatq, term_list, replicate at 2, term_list' at 2, fold_left in H.
-  rewrite (term_list_replicate (S n) termincr termnop) in H.
+  unfold termnatq, termlist, replicate at 2, termlist' at 2, fold_left in H.
+  rewrite (termlist_replicate (S n) termincr termnop) in H.
   inversion H.
   f_equal.
   apply IHn.
-  unfold termnatq, term_list in *.
-  repeat erewrite term_list_replicate in *.
+  unfold termnatq, termlist in *.
+  repeat erewrite termlist_replicate in *.
   inversion H.
   auto.
 Qed.
 
 Lemma termnat_eqmap : forall (n m : nat) (t : term),
-  termnat n t -> termnat m t -> n = m.
+  termnat_spec n t -> termnat_spec m t -> n = m.
   intros.
   assert
-    (([], replicate n term_pop) |=>*' ([], replicate m term_pop) \/
-     ([], replicate m term_pop) |=>*' ([], replicate n term_pop)).
+    (([], replicate n termpop) |=>*' ([], replicate m termpop) \/
+     ([], replicate m termpop) |=>*' ([], replicate n termpop)).
     repeat erewrite <- evalrtc_is_evalrtc'.
-    eapply (evalrtc_confluence ([ term_pop ], [ t ])).
+    apply (evalrtc_confluence ([ termpop ], [ t ])).
     evalpartial H.
     erewrite app_nil_r.
     evalauto.
     evalpartial H0.
     erewrite app_nil_r.
     evalauto.
-  assert (replicate n term_pop = replicate m term_pop).
+  assert (replicate n termpop = replicate m termpop).
     destruct H1 ; destruct n ; destruct m ; inversion H1 ;
       (auto || inversion H2 || simpl ; f_equal ; auto).
   clear H H0 H1.
-  revert m H2 ; induction n ; intro ; destruct m ; simpl ; intros.
-  auto.
-  congruence.
-  congruence.
-  f_equal ; apply IHn ; congruence.
+  revert m H2 ; induction n ; intro ; destruct m ; simpl ; intros ;
+    (auto || congruence || f_equal ; apply IHn ; congruence).
 Qed.
 
 Definition termnatq_succ : term :=
-  term_list [ term_push ; termincr ; term_cons ].
+  termlist [ termpush ; termincr ; termcons ].
 
 Lemma eval_termnatq_succ : forall (n : nat) (vs ps : stack),
   (termnatq n :: vs, termnatq_succ :: ps) |=>* (termnatq (S n) :: vs, ps).
   intros.
   evalauto.
   rtcequal.
-  unfold termnat_term, termnatq, term_list.
-  erewrite term_list_replicate.
+  unfold termnat, termnatq, termlist.
+  erewrite termlist_replicate.
   simpl ; unfold flip ; f_equal.
-  apply eq_sym, term_list_replicate.
+  apply eq_sym, termlist_replicate.
 Qed.
 
 Lemma eval_termnatq_succ_replicate : forall (n m : nat) (vs ps : stack),
@@ -144,32 +141,32 @@ Lemma eval_termnatq_succ_replicate : forall (n m : nat) (vs ps : stack),
 Qed.
 
 Definition termnat_succ : term :=
-  term_list [ termnat_quote ; termnatq_succ ; termnat_unquote ].
+  termlist [ termnat_quote ; termnatq_succ ; termnat_unquote ].
 
 Lemma eval_termnat_succ :
-  forall (n : nat) (t : term) (vs ps : stack), termnat n t ->
-    (t :: vs, termnat_succ :: ps) |=>* (termnat_term (S n) :: vs, ps).
+  forall (n : nat) (t : term) (vs ps : stack), termnat_spec n t ->
+    (t :: vs, termnat_succ :: ps) |=>* (termnat (S n) :: vs, ps).
   intros.
-  evalpartial eval_term_list.
+  evalpartial eval_termlist.
   evalpartial' eval_termnat_quote.
   apply H.
   evalpartial eval_termnatq_succ.
   evalauto.
 Qed.
 
-Lemma termnat_succ_prop :
-  forall (n : nat) (t1 : term) (vs ps : stack), termnat n t1 ->
-    exists t2 : term, termnat (S n) t2 /\
+Lemma termnat_succ_proof :
+  forall (n : nat) (t1 : term) (vs ps : stack), termnat_spec n t1 ->
+    exists t2 : term, termnat_spec (S n) t2 /\
       (t1 :: vs, termnat_succ :: ps) |=>* (t2 :: vs, ps).
   intros.
-  exists (termnat_term (S n)).
+  exists (termnat (S n)).
   split.
-  apply eval_termnat_term.
+  apply eval_termnat.
   apply eval_termnat_succ ; auto.
 Qed.
 
 Definition termnatq_add : term :=
-  term_list [ term_push ; termincr ; term_swap ; term_exec ; term_pop ].
+  termlist [ termpush ; termincr ; termswap ; termexec ; termpop ].
 
 Lemma eval_termnatq_add : forall (n m : nat) (vs ps : stack),
   (termnatq m :: termnatq n :: vs, termnatq_add :: ps) |=>*
@@ -179,19 +176,19 @@ Lemma eval_termnatq_add : forall (n m : nat) (vs ps : stack),
   evalpartial eval_termnatq.
   evalauto.
   unfold termnatq.
-  erewrite <- app_term_list, replicate_app.
+  erewrite <- app_termlist, replicate_app.
   evalauto.
 Qed.
 
-Definition termnat_add : term := term_list
-  [ termnat_quote ; term_swap ;
-    term_push ; termnatq_succ ; term_swap ; term_exec ; termnat_unquote ].
+Definition termnat_add : term := termlist
+  [ termnat_quote ; termswap ;
+    termpush ; termnatq_succ ; termswap ; termexec ; termnat_unquote ].
 
 Lemma eval_termnat_add : forall (n m : nat) (t1 t2 : term) (vs ps : stack),
-  termnat n t1 -> termnat m t2 ->
-    (t2 :: t1 :: vs, termnat_add :: ps) |=>* (termnat_term (n + m) :: vs, ps).
+  termnat_spec n t1 -> termnat_spec m t2 ->
+    (t2 :: t1 :: vs, termnat_add :: ps) |=>* (termnat (n + m) :: vs, ps).
   intros.
-  evalpartial eval_term_list.
+  evalpartial eval_termlist.
   evalpartial' eval_termnat_quote.
   apply H0.
   evalauto.
@@ -200,37 +197,37 @@ Lemma eval_termnat_add : forall (n m : nat) (t1 t2 : term) (vs ps : stack),
   apply eval_termnat_unquote.
 Qed.
 
-Lemma termnat_add_prop : forall (n m : nat) (t1 t2 : term) (vs ps : stack),
-  termnat n t1 -> termnat m t2 ->
-    exists t3 : term, termnat (n + m) t3 /\
+Lemma termnat_add_proof : forall (n m : nat) (t1 t2 : term) (vs ps : stack),
+  termnat_spec n t1 -> termnat_spec m t2 ->
+    exists t3 : term, termnat_spec (n + m) t3 /\
       (t2 :: t1 :: vs, termnat_add :: ps) |=>* (t3 :: vs, ps).
   intros.
   eexists.
   split.
-  apply eval_termnat_term.
+  apply eval_termnat.
   apply eval_termnat_add ; auto.
 Qed.
 
-Definition termnatq_mult : term := term_list
-  [ term_push ; termnop ; term_push ; term_push ; term_cons ; term_snoc ;
-    term_push ; termnatq_add ; term_cons ; term_quote ;
-    term_push ; termnatq 0 ; term_quote ; term_snoc ;
-    term_swap ; termnat_unquote ; term_cons ; term_exec ].
+Definition termnatq_mult : term := termlist
+  [ termpush ; termnop ; termpush ; termpush ; termcons ; termsnoc ;
+    termpush ; termnatq_add ; termcons ; termquote ;
+    termpush ; termnatq 0 ; termquote ; termsnoc ;
+    termswap ; termnat_unquote ; termcons ; termexec ].
 
 Lemma eval_termnatq_mult : forall (n m : nat) (vs ps : stack),
   (termnatq m :: termnatq n :: vs, termnatq_mult :: ps) |=>*
     (termnatq (n * m) :: vs, ps).
   intros.
   do 126 evalstep.
-  evalpartial eval_termnat_term.
+  evalpartial eval_termnat.
   assert (forall (a : nat), (termnatq a :: vs,
-    replicate n (term_list [ term_push ; termnatq m ; termnatq_add ]) ++ ps)
+    replicate n (termlist [ termpush ; termnatq m ; termnatq_add ]) ++ ps)
       |=>* (termnatq (a + n * m) :: vs, ps)).
     induction n ; intros.
     replace (a + 0 * m) with a by omega.
     evalauto.
     simpl.
-    evalpartial eval_term_list.
+    evalpartial eval_termlist.
     evalstep.
     evalpartial eval_termnatq_add.
     replace (a + (m + n * m)) with ((a + m) + n * m) by omega.
@@ -238,15 +235,15 @@ Lemma eval_termnatq_mult : forall (n m : nat) (vs ps : stack),
   evalpartial (H 0) ; evalauto.
 Qed.
 
-Definition termnat_mult : term := term_list
-  [ termnat_quote ; term_swap ; termnat_quote ; term_swap ;
+Definition termnat_mult : term := termlist
+  [ termnat_quote ; termswap ; termnat_quote ; termswap ;
     termnatq_mult ; termnat_unquote ].
 
 Lemma eval_termnat_mult : forall (n m : nat) (t1 t2 : term) (vs ps : stack),
-  termnat n t1 -> termnat m t2 ->
-    (t2 :: t1 :: vs, termnat_mult :: ps) |=>* (termnat_term (n * m) :: vs, ps).
+  termnat_spec n t1 -> termnat_spec m t2 ->
+    (t2 :: t1 :: vs, termnat_mult :: ps) |=>* (termnat (n * m) :: vs, ps).
   intros.
-  evalpartial eval_term_list.
+  evalpartial eval_termlist.
   evalpartial' eval_termnat_quote.
   apply H0.
   evalstep.
